start proving that parser doesn't return LeftRecursion for non-left-recursive grammars

coq/Parser_error_free_termination.v
@@ -1,7 +1,9 @@
+Require Import List.
 Require Import GallStar.Defs.
 Require Import GallStar.Lex.
 Require Import GallStar.Parser.
 Require Import GallStar.Tactics.
+Import ListNotations.
 
 (* The parser never reaches an invalid state;
    i.e., impossible states really are impossible *)
@@ -60,13 +62,184 @@ Qed.
 (* TODO -- The parser only returns a LeftRecursion error
    if the grammar is left-recursive *)
 
+Inductive nullable_sym (g : grammar) : symbol -> Prop :=
+| NullableSym : forall x ys,
+    In (x, ys) g
+    -> nullable_gamma g ys
+    -> nullable_sym g (NT x)
+with nullable_gamma (g : grammar) : list symbol -> Prop :=
+     | NullableNil  : nullable_gamma g []
+     | NullableCons : forall hd tl,
+         nullable_sym g hd
+         -> nullable_gamma g tl
+         -> nullable_gamma g (hd :: tl).
+
+Inductive nullable_gamma' (g : grammar) : list symbol -> Prop :=
+| NullableNil'  : 
+    nullable_gamma' g []
+| NullableCons' : 
+    forall x ys tl,
+      In (x, ys) g
+      -> nullable_gamma' g ys
+      -> nullable_gamma' g tl
+      -> nullable_gamma' g (NT x :: tl).
+
+Inductive nullable_path (g : grammar) :
+  symbol -> symbol -> Prop :=
+| DirectPath : forall x z gamma pre suf,
+    In (x, gamma) g
+    -> gamma = pre ++ NT z :: suf
+    -> nullable_gamma g pre
+    -> nullable_path g (NT x) (NT z)
+| IndirectPath : forall x y z gamma pre suf,
+    In (x, gamma) g
+    -> gamma = pre ++ NT y :: suf
+    -> nullable_gamma g pre
+    -> nullable_path g (NT y) (NT z)
+    -> nullable_path g (NT x) (NT z).
+
+Inductive path (g : grammar) :
+  symbol -> symbol -> Prop :=
+| DirectPath' : forall x z gamma pre suf,
+    In (x, gamma) g
+    -> gamma = pre ++ NT z :: suf
+    -> path g (NT x) (NT z)
+| IndirectPath' : forall x y z gamma pre suf,
+    In (x, gamma) g
+    -> gamma = pre ++ NT y :: suf
+    -> path g (NT y) (NT z)
+    -> path g (NT x) (NT z).
+
+Hint Constructors nullable_path.
+
+Definition left_recursive g sym :=
+  nullable_path g sym sym.
+
+Definition no_left_recursion g :=
+  forall (x : nonterminal),
+    ~ left_recursive g (NT x).
+
+Inductive nullable_frames_path (g : grammar) : nonterminal -> nonterminal -> list frame -> Prop :=
+| NFP : 
+    forall top_fr mid_frs bot_fr x y suf suf',
+      bot_fr.(loc).(rsuf) = NT x :: suf
+      -> List.Forall (fun mf => nullable_gamma g mf.(loc).(rpre)) mid_frs
+      -> nullable_gamma g top_fr.(loc).(rpre)
+      -> top_fr.(loc).(rsuf) = NT y :: suf'
+      -> nullable_frames_path g x y (top_fr :: mid_frs ++ [bot_fr]).
+
+Lemma multistep_left_recursion_detection_sound :
+  forall (g : grammar)
+         (tri : nat * nat * nat)
+         (a : Acc lex_nat_triple tri)
+         (av : NtSet.t) 
+         fr frs
+         (ts : list token)
+         (a' : Acc lex_nat_triple (meas g (Pst av (fr, frs) ts)))
+         (x : nonterminal),
+    stack_wf g (fr, frs)
+    -> tri = meas g (Pst av (fr, frs) ts)
+    -> multistep g (Pst av (fr, frs) ts) a' = Error (LeftRecursion x)
+    -> (~ NtSet.In x av
+        /\ (exists pre s suf,
+               fr.(loc).(rpre) ++ fr.(loc).(rsuf) = pre ++ s :: suf
+               /\ nullable_gamma g pre
+               /\ (s = NT x \/ nullable_path g s (NT x))))
+       \/ left_recursive g (NT x).
+Proof.
+  intros g tri a'.
+  induction a' as [tri hlt IH].
+  intros av fr frs ts a x hw heq hm; subst.
+  apply multistep_left_recursion_cases in hm.
+  destruct hm as [hs | hm].
+  - admit.
+  - destruct hm as [[av' (fr', frs') ts'] [a'' [hs hm]]].
+    eapply IH in hm; clear IH; clear hlt; auto.
+    + destruct hm as [hnin | hlr]; auto.
+      clear a a''.
+      destruct hnin as [hnin [pre [s [suf [heq [hng hor]]]]]]; subst.
+      destruct hor as [heq' | hnp]; subst.
+      * unfold step in hs; repeat dmeq heq; tc; inv hs; subst; sis.
+        -- rewrite <- app_assoc in heq.
+           simpl in *.
+           inv hw.
+           destruct (NF.eq_dec x n); subst.
+           ++ ND.fsetdec.
+           ++ left. split.
+              ** ND.fsetdec.
+              ** rewrite app_nil_r in *.
+Abort.           
+
+Lemma multistep_left_recursion_detection_sound :
+  forall (g : grammar)
+         (tri : nat * nat * nat)
+         (a : Acc lex_nat_triple tri)
+         (av : NtSet.t) 
+         fr frs
+         (ts : list token)
+         (a' : Acc lex_nat_triple (meas g (Pst av (fr, frs) ts)))
+         (x : nonterminal),
+    tri = meas g (Pst av (fr, frs) ts)
+    -> multistep g (Pst av (fr, frs) ts) a' = Error (LeftRecursion x)
+    -> (exists fr' pre s suf,
+           In fr' (fr :: frs)
+           /\ fr'.(loc).(rsuf) = pre ++ s :: suf
+           /\ ~ NtSet.In x av
+           /\ (s = NT x
+               \/ nullable_path g s (NT x)))
+       \/ left_recursive g (NT x).
+Proof.
+  intros g tri a'.
+  induction a' as [tri hlt IH].
+  intros av fr frs ts a x heq hm; subst.
+  apply multistep_left_recursion_cases in hm.
+  destruct hm as [hs | hm].
+  - admit.
+  - destruct hm as [[av' (fr', frs') ts'] [a'' [hs hm]]].
+    eapply IH in hm; clear IH; clear hlt; eauto.
+    + destruct hm as [hex | hlr]; auto.
+      destruct hex as [fr'' [pre [s [suf [hin [heq [hnin hor]]]]]]].
+      destruct hor as [heq' | hnp]; subst.
+      * destruct hin as [hh | ht]; subst.
+Abort.
+
+Lemma multistep_left_recursion_detection_sound :
+  forall g av stk ts a x,
+    multistep g (Pst av stk ts) a = Error (LeftRecursion x)
+    -> (In x (lhss g) /\ ~ NtSet.In x av)
+       \/ left_recursive g (NT x).
+Admitted.
+
+Lemma parse_left_recursion_detection_sound :
+  forall g ss ts x,
+    parse g ss ts = Error (LeftRecursion x)
+    -> left_recursive g (NT x).
+Proof.
+  intros g ss ts x hp; unfold parse in hp.
+  apply multistep_left_recursion_detection_sound in hp.
+  destruct hp as [[hi hn] | hlr]; auto.
+  apply in_lhss_in_allNts in hi; firstorder.
+Qed.
+  
+Lemma parser_doesn't_report_nonexistent_left_recursion :
+  forall (g  : grammar)
+         (ss : list symbol)
+         (ts : list token)
+         (x  : nonterminal),
+    no_left_recursion g
+    -> ~ parse g ss ts = Error (LeftRecursion x).
+Proof.
+  intros g ss ts x hn; unfold not; intros hp.
+  apply parse_left_recursion_detection_sound in hp; firstorder.
+Qed.
 
 Theorem parser_terminates_without_error :
   forall (g  : grammar)
          (ss : list symbol)
          (ts : list token)
          (e  : error_type),
-    ~ parse g ss ts = Error e.
+    no_left_recursion g
+    -> ~ parse g ss ts = Error e.
 Proof.
   intros g ss ts e; unfold not; intros hp.
   destruct e.
@@ -75,5 +248,5 @@ Proof.
   - (* prediction error case *)
     admit.
   - (* left recursion case *)
-    admit.
+    apply parser_doesn't_report_nonexistent_left_recursion; auto.
 Admitted.
